Add documentation and tests (more needed)
Signed-off-by: Adrian Palacios <accorell@amazon.com>

cedar-lean/Cedar/Spec/Ext/Datetime.lean
@@ -23,6 +23,60 @@ namespace Cedar.Spec.Ext
 
 open Cedar.Data
 
+namespace Datetime
+
+/--
+  A datetime value is measured in milliseconds and constructed from a datetime string.
+  A datetime string must be of one of the forms:
+  - `YYYY-MM-DD` (date only)
+  - `YYYY-MM-DDThh:mm:ssZ` (UTC)
+  - `YYYY-MM-DDThh:mm:ss.SSSZ` (UTC with millisecond precision)
+  - `YYYY-MM-DDThh:mm:ss(+|-)hhmm` (With timezone offset in hours and minutes)
+  - `YYYY-MM-DDThh:mm:ss.SSS(+|-)hhmm` (With timezone offset in hours and minutes and millisecond precision)
+-/
+abbrev Datetime := Int64
+
+def DateOnly : Std.Time.GenericFormat .any := datespec("uuuu-MM-dd")
+def DateUTC : Std.Time.GenericFormat .any := datespec("uuuu-MM-dd'T'HH:mm:ss'Z'")
+def DateUTCWithMillis : Std.Time.GenericFormat .any := datespec("uuuu-MM-dd'T'HH:mm:ss.SSS'Z'")
+def DateWithOffset : Std.Time.GenericFormat .any := datespec("uuuu-MM-dd'T'HH:mm:ssxx")
+def DateWithOffsetAndMillis : Std.Time.GenericFormat .any := datespec("uuuu-MM-dd'T'HH:mm:ss.SSSxx")
+
+abbrev datetime? := Int64.ofInt?
+
+def parse (str: String) : Option Datetime :=
+  let parseFun := match str.length with
+  | 10 => DateOnly.parse
+  | 20 => DateUTC.parse
+  | 24 => if str.get? ⟨23⟩ == some 'Z'
+          then DateUTCWithMillis.parse
+          else DateWithOffset.parse
+  | 28 => DateWithOffsetAndMillis.parse
+  | _ => (fun _ => Except.error "invalid string length")
+
+  let datetime := parseFun str
+  match datetime with
+  | Except.ok val => datetime? val.toTimestamp.toMillisecondsSinceUnixEpoch.toInt
+  | _ => none
+
+#eval DateOnly.parse "2022-10-10"
+#eval DateUTC.parse "2022-10-10T00:00:00Z"
+#eval DateUTCWithMillis.parse "2022-10-10T03:35:00.001Z"
+#eval DateWithOffset.parse "2022-10-10T03:35:00+0500"
+#eval DateWithOffsetAndMillis.parse "2022-10-10T03:35:00.000+0500"
+
+#eval parse "2022-10-10"
+#eval parse "2022-10-10T00:00:00Z"
+#eval parse "2022-10-10T03:35:00.001Z"
+#eval parse "2022-10-10T03:35:00+0500"
+#eval parse "2022-10-10T03:35:00.000+0500"
+
+#eval "2022-10-10".length
+#eval "2022-10-10T00:00:00Z".length
+#eval "2022-10-10T03:35:00.001Z".length
+#eval "2022-10-10T03:35:00+05:00".length
+#eval "2022-10-10T03:35:00.000+05:00".length
+-- #eval (parse "1969-12-31") == (Int64.ofInt (-86400000 :Int))
 /--
   A duration value is measured in milliseconds and constructed from a duration string.
   A duration string is a concatenated sequence of quantity-unit pairs where the quantity
@@ -40,8 +94,6 @@ open Cedar.Data
   A duration may be negative. Negative duration strings must begin with `-`.
 -/
 abbrev Duration := Int64
-
-namespace Datetime
 
 def MILLISECONDS_PER_SECOND: Int := 1000
 def MILLISECONDS_PER_MINUTE: Int := 60000
@@ -113,53 +165,5 @@ def Duration.parse (str : String) : Option Duration :=
 deriving instance Repr for Duration
 
 abbrev duration := Duration.parse
-
-abbrev Datetime := Int64
-
--- /-
---   * `YYYY-MM-DD` (date only)
---   * `YYYY-MM-DDThh:mm:ssZ"` (UTC)
---   * `"YYYY-MM-DDThh:mm:ss.SSSZ"` (UTC with millisecond precision)
---   * `"YYYY-MM-DDThh:mm:ss(+|-)hhmm"` (With timezone offset in hours and minutes)
---   * `"YYYY-MM-DDThh:mm:ss.SSS(+|-)hhmm"` (With timezone offset in hours and minutes and millisecond precision)
--- -/
-def DateOnly : Std.Time.GenericFormat .any := datespec("uuuu-MM-dd")
-def DateUTC : Std.Time.GenericFormat .any := datespec("uuuu-MM-dd'T'HH:mm:ss'Z'")
-def DateUTCWithMillis : Std.Time.GenericFormat .any := datespec("uuuu-MM-dd'T'HH:mm:ss.SSS'Z'")
-def DateWithOffset : Std.Time.GenericFormat .any := datespec("uuuu-MM-dd'T'HH:mm:ssxxx")
-def DateWithOffsetAndMillis : Std.Time.GenericFormat .any := datespec("uuuu-MM-dd'T'HH:mm:ss.SSSxxx")
-
-def parse (str: String) : Option Datetime :=
-  let parseFun := match str.length with
-  | 10 => DateOnly.parse
-  | 20 => DateUTC.parse
-  | 24 => DateUTCWithMillis.parse
-  | 25 => DateWithOffset.parse
-  | 29 => DateWithOffsetAndMillis.parse
-  | _ => (fun _ => Except.error "invalid string length")
-
-  let datetime := parseFun str
-  match datetime with
-  | Except.ok val => Int64.ofInt? val.toTimestamp.toMillisecondsSinceUnixEpoch.toInt
-  | _ => none
-
-#eval DateOnly.parse "2022-10-10"
-#eval DateUTC.parse "2022-10-10T00:00:00Z"
-#eval DateUTCWithMillis.parse "2022-10-10T03:35:00.001Z"
-#eval DateWithOffset.parse "2022-10-10T03:35:00+05:00"
-#eval DateWithOffsetAndMillis.parse "2022-10-10T03:35:00.000+05:00"
-
-#eval parse "2022-10-10"
-#eval (parse "1969-12-31") == (Int64.ofInt (-86400000 :Int))
-#eval parse "2022-10-10T00:00:00Z"
-#eval parse "2022-10-10T03:35:00.001Z"
-#eval parse "2022-10-10T03:35:00+05:00"
-#eval parse "2022-10-10T03:35:00.000+05:00"
-
-#eval "2022-10-10".length
-#eval "2022-10-10T00:00:00Z".length
-#eval "2022-10-10T03:35:00.001Z".length
-#eval "2022-10-10T03:35:00+05:00".length
-#eval "2022-10-10T03:35:00.000+05:00".length
 
 end Datetime
