cedar-lean/UnitTest/Datetime.lean
@@ -23,79 +23,111 @@ namespace UnitTest.Datetime
 
 open Cedar.Spec.Ext.Datetime
 
-theorem test1 : toString ((Duration.parse "1ms").get!) = "1" := by native_decide
-theorem test2 : toString ((Duration.parse "1s").get!) = "1000" := by native_decide
-theorem test3 : toString ((Duration.parse "1m").get!) = "60000" := by native_decide
-theorem test4 : toString ((Duration.parse "1h").get!) = "360000" := by native_decide
-theorem test5 : toString ((Duration.parse "1d").get!) = "86400000" := by native_decide
-theorem test6 : toString ((Duration.parse "1d2h3m4s5ms").get!) = "87304005" := by native_decide
-theorem test7 : toString ((Duration.parse "2d12h").get!) = "177120000" := by native_decide
-theorem test8 : toString ((Duration.parse "3m30s").get!) = "210000" := by native_decide
-theorem test9 : toString ((Duration.parse "1h30m45s").get!) = "2205000" := by native_decide
-theorem test10 : toString ((Duration.parse "2d5h20m").get!) = "175800000" := by native_decide
-theorem test11 : toString ((Duration.parse "-1d12h").get!) = "-90720000" := by native_decide
-theorem test12 : toString ((Duration.parse "-3h45m").get!) = "-3780000" := by native_decide
-theorem test13 : toString ((Duration.parse "1d1ms").get!) = "86400001" := by native_decide
-theorem test14 : toString ((Duration.parse "59m59s999ms").get!) = "3599999" := by native_decide
-theorem test15 : toString ((Duration.parse "23h59m59s999ms").get!) = "11879999" := by native_decide
-theorem test16 : toString ((Duration.parse "0d0h0m0s0ms").get!) = "0" := by native_decide
 
-private def testValid (str : String) (rep : Int) : TestCase IO :=
+theorem testDatetime1 : toString ((parse "2022-10-10").get!) = "1665360000000" := by native_decide
+theorem testDatetime2 : toString ((parse "1969-12-31").get!) = "-86400000" := by native_decide
+
+private def testValidDatetime (str : String) (rep : Int) : TestCase IO :=
+  test str ⟨λ _ => checkEq (parse str) (datetime? rep)⟩
+
+def testsForValidDatetimeStrings :=
+  suite "Datetime.parse for valid strings"
+  [
+    testValidDatetime "1970-01-01" 0,
+    testValidDatetime "2024-10-15" 1728950400000,
+    testValidDatetime "2024-10-15T11:38:02Z" 1728992282000,
+    testValidDatetime "2024-10-15T11:38:02.101Z" 1728992282101,
+    testValidDatetime "2024-10-15T11:38:02.101-1134" 1729033922101,
+    testValidDatetime "2024-10-15T11:38:02.101+1134" 1728950642101,
+    testValidDatetime "2024-10-15T11:38:02+1134" 1728950642000,
+    testValidDatetime "2024-10-15T11:38:02-1134" 1729033922000,
+    testValidDatetime "2016-12-31T23:59:60Z" 1483228800000, -- the last leap second
+    testValidDatetime "2017-01-01" 1483228800000, -- same date without leap second
+  ]
+
+private def testInvalidDatetime (str : String) (msg : String) : TestCase IO :=
+  test s!"{str} [{msg}]" ⟨λ _ => checkEq (Duration.parse str) .none⟩
+
+def testsForInvalidDatetimeStrings :=
+  suite "Datetime.parse for invalid strings"
+  [
+    testInvalidDatetime "1970-01-00" "does not exist",
+  ]
+
+theorem testDuration1 : toString ((Duration.parse "1ms").get!) = "1" := by native_decide
+theorem testDuration2 : toString ((Duration.parse "1s").get!) = "1000" := by native_decide
+theorem testDuration3 : toString ((Duration.parse "1m").get!) = "60000" := by native_decide
+theorem testDuration4 : toString ((Duration.parse "1h").get!) = "360000" := by native_decide
+theorem testDuration5 : toString ((Duration.parse "1d").get!) = "86400000" := by native_decide
+theorem testDuration6 : toString ((Duration.parse "1d2h3m4s5ms").get!) = "87304005" := by native_decide
+theorem testDuration7 : toString ((Duration.parse "2d12h").get!) = "177120000" := by native_decide
+theorem testDuration8 : toString ((Duration.parse "3m30s").get!) = "210000" := by native_decide
+theorem testDuration9 : toString ((Duration.parse "1h30m45s").get!) = "2205000" := by native_decide
+theorem testDuration10 : toString ((Duration.parse "2d5h20m").get!) = "175800000" := by native_decide
+theorem testDuration11 : toString ((Duration.parse "-1d12h").get!) = "-90720000" := by native_decide
+theorem testDuration12 : toString ((Duration.parse "-3h45m").get!) = "-3780000" := by native_decide
+theorem testDuration13 : toString ((Duration.parse "1d1ms").get!) = "86400001" := by native_decide
+theorem testDuration14 : toString ((Duration.parse "59m59s999ms").get!) = "3599999" := by native_decide
+theorem testDuration15 : toString ((Duration.parse "23h59m59s999ms").get!) = "11879999" := by native_decide
+theorem testDuration16 : toString ((Duration.parse "0d0h0m0s0ms").get!) = "0" := by native_decide
+
+private def testValidDuration (str : String) (rep : Int) : TestCase IO :=
   test str ⟨λ _ => checkEq (Duration.parse str) (duration? rep)⟩
 
 def testsForValidDurationStrings :=
   suite "Duration.parse for valid strings"
   [
-    testValid "0ms" 0,
-    testValid "0d0s" 0,
-    testValid "1ms" 1,
-    testValid "1s" 1000,
-    testValid "1m" 60000,
-    testValid "1h" 360000,
-    testValid "1d" 86400000,
-    testValid "12s340ms" 12340,
-    testValid "1s234ms" 1234,
-    testValid "-1s" (-1000),
-    testValid "-4s200ms" (-4200),
-    testValid "-9s876ms" (-9876),
-    testValid "106751d23h47m16s854ms" 9223297516854,
-    testValid "-106751d23h47m16s854ms" (-9223297516854),
-    testValid "1d2h3m4s5ms" 87304005,
-    testValid "2d12h" 177120000,
-    testValid "3m30s" 210000,
-    testValid "1h30m45s" 2205000,
-    testValid "2d5h20m" 175800000,
-    testValid "-1d12h" (-90720000),
-    testValid "-3h45m" (-3780000),
-    testValid "1d1ms" 86400001,
-    testValid "59m59s999ms" 3599999,
-    testValid "23h59m59s999ms" 11879999
+    testValidDuration "0ms" 0,
+    testValidDuration "0d0s" 0,
+    testValidDuration "1ms" 1,
+    testValidDuration "1s" 1000,
+    testValidDuration "1m" 60000,
+    testValidDuration "1h" 360000,
+    testValidDuration "1d" 86400000,
+    testValidDuration "12s340ms" 12340,
+    testValidDuration "1s234ms" 1234,
+    testValidDuration "-1s" (-1000),
+    testValidDuration "-4s200ms" (-4200),
+    testValidDuration "-9s876ms" (-9876),
+    testValidDuration "106751d23h47m16s854ms" 9223297516854,
+    testValidDuration "-106751d23h47m16s854ms" (-9223297516854),
+    testValidDuration "1d2h3m4s5ms" 87304005,
+    testValidDuration "2d12h" 177120000,
+    testValidDuration "3m30s" 210000,
+    testValidDuration "1h30m45s" 2205000,
+    testValidDuration "2d5h20m" 175800000,
+    testValidDuration "-1d12h" (-90720000),
+    testValidDuration "-3h45m" (-3780000),
+    testValidDuration "1d1ms" 86400001,
+    testValidDuration "59m59s999ms" 3599999,
+    testValidDuration "23h59m59s999ms" 11879999
   ]
 
-private def testInvalid (str : String) (msg : String) : TestCase IO :=
+private def testInvalidDuration (str : String) (msg : String) : TestCase IO :=
   test s!"{str} [{msg}]" ⟨λ _ => checkEq (Duration.parse str) .none⟩
 
 def testsForInvalidDurationStrings :=
   suite "Duration.parse for invalid strings"
   [
-    testInvalid "" "empty string",
-    testInvalid "d" "unit but no amount",
-    testInvalid "1d-1s" "invalid use of -",
-    testInvalid "1d2h3m4s5ms6" "trailing amount",
-    testInvalid "1x2m3s" "invalid unit",
-    testInvalid "1.23s" "amounts must be integral",
-    testInvalid "1s1d" "invalid order",
-    testInvalid "1s1s" "repeated units",
-    testInvalid "1d2h3m4s5ms " "trailing space",
-    testInvalid " 1d2h3m4s5ms" "leading space",
-    testInvalid "1d9223372036854775807ms" "overflow",
-    testInvalid "1d92233720368547758071ms" "overflow ms",
-    testInvalid "9223372036854776s1ms" "overflow s"
+    testInvalidDuration "" "empty string",
+    testInvalidDuration "d" "unit but no amount",
+    testInvalidDuration "1d-1s" "invalid use of -",
+    testInvalidDuration "1d2h3m4s5ms6" "trailing amount",
+    testInvalidDuration "1x2m3s" "invalid unit",
+    testInvalidDuration "1.23s" "amounts must be integral",
+    testInvalidDuration "1s1d" "invalid order",
+    testInvalidDuration "1s1s" "repeated units",
+    testInvalidDuration "1d2h3m4s5ms " "trailing space",
+    testInvalidDuration " 1d2h3m4s5ms" "leading space",
+    testInvalidDuration "1d9223372036854775807ms" "overflow",
+    testInvalidDuration "1d92233720368547758071ms" "overflow ms",
+    testInvalidDuration "9223372036854776s1ms" "overflow s"
   ]
 
-def tests := [testsForValidDurationStrings, testsForInvalidDurationStrings]
+def tests := [testsForValidDatetimeStrings, testsForInvalidDatetimeStrings,
+              testsForValidDurationStrings, testsForInvalidDurationStrings]
 
 -- Uncomment for interactive debugging
--- #eval TestSuite.runAll tests
+#eval TestSuite.runAll tests
 
 end UnitTest.Datetime
